# Calculus I: Appendix-E: Derivation of the dot product and the projection vectors 

## 1) The dot product: 

- Recall, 2 intersecting vectors $u$ and $v$ together with the resultant vetcor $w$; such that, $$w = u - v$$

- From the "Law of Cosines":
$$Since, ||w||^2 = ||u||^2 + ||v||^2 - 2 * ||u|| * ||v|| * cos(\theta)$$
$$Then, cos(\theta) = (||w||^2 - ||u||^2 - ||v||^2) / -2 * ||u|| * ||v||\ Lemma\.01$$ 

$$Since, ||w|| = \sqrt{(u_x - v_x)^2 + (u_y - v_y)^2 + (u_z - v_z)^2}$$

$$||v|| = \sqrt{{v_x}^2 + {v_y}^2 + {v_z}^2}$$

$$||u|| = \sqrt{{u_x}^2 + {u_y}^2 + {u_z}^2}$$

$$||w|| = ||u-v|| = \sqrt{{u_x - v_x}^2 + {u_y - v_y}^2 + {u_z - v_z}^2}$$

$$Then, 1)\ ||v||^2 = {v_x}^2 + {v_y}^2 + {v_z}^2$$

$$ 2)\ ||u||^2 = {u_x}^2 + {u_y}^2 + {u_z}^2$$

$$ 3)\ ||w||^2 = {u_x - v_x}^2 + {u_y - v_y}^2 + {u_z - v_z}^2$$


$$Hence, cos(\theta) = u.v / ||u|| * ||v||$$
$$Thence, u.v = ||u|| * ||v|| * cos(\theta)$$

## 2) Projection vectors: 


